\documentclass[a4paper,12pt]{article}
\usepackage{problems}
\title{Problem Write-up 2}
\date{2019-09-29}

\begin{document}
    \begin{prob}
        In this problem, we will justify the equvalence \[p \leftrightarrow q \Leftrightarrow (p \to q) \wedge (q \to p).\]
        So consider the statements \(A = p \leftrightarrow q\) and \(B = (p \to q) \wedge (q \to p)\).

        \begin{enumerate}
                \item Argue if \(A\) is false, then so is \(B\). Do \textit{not} use the proposed equivalence above as part of your argument.
                \item Argue if \(B\) is false, then so is \(A\). Do \textit{not} use the proposed equivalence above as part of your argument.
                \item Explain why the two arguments in (a) and (b), taken together, justify the equivalence \(A \Leftrightarrow B\). Do this \textit{without} making any further arguments about the truth values of \(p\) and \(q\).
        \end{enumerate}
    \end{prob}

    \begin{proof}
        Here, we're asked to prove the equivalence of two statements 
    \end{proof}
\end{document}